Parameterize go_lang over an FFI
Covers the parameterization; now need to see how to prove programs using
this model, and especially to make all the heap reasoning parameterized
over an arbitrary FFI model. Then we should actually instantiate the FFI
and use it for a disk model as a test.

src/go_lang/adequacy.v
@@ -5,17 +5,17 @@ From iris.program_logic Require Export weakestpre adequacy.
 From Perennial.go_lang Require Import proofmode notation.
 Set Default Proof Using "Type".
 
-Class heapPreG Σ := HeapPreG {
+Class heapPreG `{ffi_sem: ext_semantics} Σ := HeapPreG {
   heap_preG_iris :> invPreG Σ;
   heap_preG_heap :> gen_heapPreG loc val Σ;
   heap_preG_proph :> proph_mapPreG proph_id (val * val) Σ
 }.
 
-Definition heapΣ : gFunctors := #[invΣ; gen_heapΣ loc val; proph_mapΣ proph_id (val * val)].
-Instance subG_heapPreG {Σ} : subG heapΣ Σ → heapPreG Σ.
+Definition heapΣ `{ffi_sem: ext_semantics} : gFunctors := #[invΣ; gen_heapΣ loc val; proph_mapΣ proph_id (val * val)].
+Instance subG_heapPreG `{ffi_sem: ext_semantics} {Σ} : subG heapΣ Σ → heapPreG Σ.
 Proof. solve_inG. Qed.
 
-Definition heap_adequacy Σ `{!heapPreG Σ} s e σ φ :
+Definition heap_adequacy `{ffi_sem: ext_semantics} Σ `{!heapPreG Σ} s e σ φ :
   (∀ `{!heapG Σ}, WP e @ s; ⊤ {{ v, ⌜φ v⌝ }}%I) →
   adequate s e σ (λ v _, φ v).
 Proof.
