src/go_lang/proofmode.v
@@ -7,11 +7,11 @@ From Perennial.go_lang Require Import notation.
 Set Default Proof Using "Type".
 Import uPred.
 
-Lemma tac_wp_expr_eval `{!heapG Σ} Δ s E Φ e e' :
+Lemma tac_wp_expr_eval `{ffi_sem: ext_semantics} `{!heapG Σ} Δ s E Φ e e' :
   (∀ (e'':=e'), e = e'') →
   envs_entails Δ (WP e' @ s; E {{ Φ }}) → envs_entails Δ (WP e @ s; E {{ Φ }}).
 Proof. by intros ->. Qed.
-Lemma tac_twp_expr_eval `{!heapG Σ} Δ s E Φ e e' :
+Lemma tac_twp_expr_eval `{ffi_sem: ext_semantics} `{!heapG Σ} Δ s E Φ e e' :
   (∀ (e'':=e'), e = e'') →
   envs_entails Δ (WP e' @ s; E [{ Φ }]) → envs_entails Δ (WP e @ s; E [{ Φ }]).
 Proof. by intros ->. Qed.
@@ -28,7 +28,7 @@ Tactic Notation "wp_expr_eval" tactic(t) :=
   | _ => fail "wp_expr_eval: not a 'wp'"
   end.
 
-Lemma tac_wp_pure `{!heapG Σ} Δ Δ' s E e1 e2 φ n Φ :
+Lemma tac_wp_pure `{ffi_sem: ext_semantics} `{!heapG Σ} Δ Δ' s E e1 e2 φ n Φ :
   PureExec φ n e1 e2 →
   φ →
   MaybeIntoLaterNEnvs n Δ Δ' →
@@ -38,7 +38,7 @@ Proof.
   rewrite envs_entails_eq=> ??? HΔ'. rewrite into_laterN_env_sound /=.
   rewrite HΔ' -lifting.wp_pure_step_later //.
 Qed.
-Lemma tac_twp_pure `{!heapG Σ} Δ s E e1 e2 φ n Φ :
+Lemma tac_twp_pure `{ffi_sem: ext_semantics} `{!heapG Σ} Δ s E e1 e2 φ n Φ :
   PureExec φ n e1 e2 →
   φ →
   envs_entails Δ (WP e2 @ s; E [{ Φ }]) →
@@ -47,10 +47,10 @@ Proof.
   rewrite envs_entails_eq=> ?? ->. rewrite -total_lifting.twp_pure_step //.
 Qed.
 
-Lemma tac_wp_value `{!heapG Σ} Δ s E Φ v :
+Lemma tac_wp_value `{ffi_sem: ext_semantics} `{!heapG Σ} Δ s E Φ v :
   envs_entails Δ (Φ v) → envs_entails Δ (WP (Val v) @ s; E {{ Φ }}).
 Proof. rewrite envs_entails_eq=> ->. by apply wp_value. Qed.
-Lemma tac_twp_value `{!heapG Σ} Δ s E Φ v :
+Lemma tac_twp_value `{ffi_sem: ext_semantics} `{!heapG Σ} Δ s E Φ v :
   envs_entails Δ (Φ v) → envs_entails Δ (WP (Val v) @ s; E [{ Φ }]).
 Proof. rewrite envs_entails_eq=> ->. by apply twp_value. Qed.
 
@@ -140,12 +140,12 @@ Tactic Notation "wp_inj" := wp_pure (InjL _) || wp_pure (InjR _).
 Tactic Notation "wp_pair" := wp_pure (Pair _ _).
 Tactic Notation "wp_closure" := wp_pure (Rec _ _ _).
 
-Lemma tac_wp_bind `{!heapG Σ} K Δ s E Φ e f :
+Lemma tac_wp_bind `{ffi_sem: ext_semantics} `{!heapG Σ} K Δ s E Φ e f :
   f = (λ e, fill K e) → (* as an eta expanded hypothesis so that we can `simpl` it *)
   envs_entails Δ (WP e @ s; E {{ v, WP f (Val v) @ s; E {{ Φ }} }})%I →
   envs_entails Δ (WP fill K e @ s; E {{ Φ }}).
 Proof. rewrite envs_entails_eq=> -> ->. by apply: wp_bind. Qed.
-Lemma tac_twp_bind `{!heapG Σ} K Δ s E Φ e f :
+Lemma tac_twp_bind `{ffi_sem: ext_semantics} `{!heapG Σ} K Δ s E Φ e f :
   f = (λ e, fill K e) → (* as an eta expanded hypothesis so that we can `simpl` it *)
   envs_entails Δ (WP e @ s; E [{ v, WP f (Val v) @ s; E [{ Φ }] }])%I →
   envs_entails Δ (WP fill K e @ s; E [{ Φ }]).
@@ -176,7 +176,7 @@ Tactic Notation "wp_bind" open_constr(efoc) :=
 
 (** Heap tactics *)
 Section heap.
-Context `{!heapG Σ}.
+Context `{ffi_sem: ext_semantics} `{!heapG Σ}.
 Implicit Types P Q : iProp Σ.
 Implicit Types Φ : val → iProp Σ.
 Implicit Types Δ : envs (uPredI (iResUR Σ)).
